first pass on getline

bedrock2/src/bedrock2Examples/ct.v
@@ -42,3 +42,214 @@ Lemma div3329_vt : program_logic_goal_for_function! div3329_vartime.
 Proof.
   repeat (straightline || eexists).
 Qed.
+
+(* Mon Jul  1 14:14:15 EDT 2024 *)
+
+Import Byte.
+Definition getchar_event c : io_event :=
+  ((Interface.map.empty, "getchar", []), (Interface.map.empty, [word.of_Z (byte.unsigned c)])).
+Instance ctspec_of_getchar : spec_of "getchar" :=
+  fun functions => forall k, exists k_, forall t m,
+      WeakestPrecondition.call functions "getchar" k t m []
+        (fun k' t' m' rets => exists c, rets = [word.of_Z (byte.unsigned c)] /\ k' = k_ /\ m' = m /\
+        t' = cons (getchar_event c) t ).
+
+Definition getline := func! (dst, n) ~> n {
+  i = $0;
+  c = $0;
+  while (i < n) {
+    unpack! c = getchar();
+    if (c == $0x0a) { n = i }
+    else { store1(dst + i, c); i = i + $1 }
+  }
+}.
+
+Local Notation "xs $@ a" := (Array.array Separation.ptsto (word.of_Z 1) a xs) (at level 10, format "xs $@ a").
+Local Infix "*" := Separation.sep.
+Local Infix "*" := Separation.sep : type_scope.
+
+Definition getline_io bs := getchar_event Byte.x0a :: map getchar_event (rev bs).
+
+Instance ctspec_of_getline : spec_of "getline" :=
+  fun functions => forall k, exists f, forall (dst n : word) d t m R,
+  (d$@dst * R) m -> length d = n :> Z ->
+      WeakestPrecondition.call functions "getline" k t m [dst; n]
+        (fun k' t' m' rets => exists bs es l, rets = [l] /\ k' = f l /\
+        (bs$@dst * es$@(word.add dst l) * R) m' /\
+        length bs = l :> Z /\
+        length bs + length es = n :> Z /\
+        (* TODO: handle case where buffer is full and final newline is not read. possibly just as an error. *)
+        t' = getline_io bs ++ t).
+
+(* Mon Jul  1 14:24:28 EDT 2024 *)
+
+Require Coq.Program.Wf.
+Import Separation SeparationLogic.
+
+Lemma getline_ct : program_logic_goal_for_function! getline.
+Proof.
+  repeat straightline.
+
+  refine ((Loops.tailrec_earlyout
+    (HList.polymorphic_list.cons (list byte)
+    (HList.polymorphic_list.cons (_ -> Prop)
+    HList.polymorphic_list.nil))
+    ["dst";"n";"i";"c"])
+    (fun (v:nat) es R k t m  dst_ n_ i c => PrimitivePair.pair.mk (
+      n_ = n /\ dst_ = dst /\ v = i :> Z /\
+      (* TODO: i <= n *)
+      (es$@(word.add dst i) * R) m /\ length es = word.sub n i :> Z
+    )
+    (fun                K T M DST N I C => DST = dst /\
+      exists bs ES, (bs$@(word.add dst i) * ES$@(word.add dst I) * R) M /\ I = N /\
+      length bs = word.sub I i :> Z /\
+      length ES = word.sub n I :> Z /\
+      (* TODO: N <= n *)
+      T = getline_io bs ++ t
+    ))
+    (fun i j : nat => j < i <= n)%Z
+    _ _ _ _ _ _ _);
+    cbn [HList.hlist.foralls HList.tuple.foralls
+         HList.hlist.existss HList.tuple.existss
+         HList.hlist.apply  HList.tuple.apply
+         HList.hlist
+         List.repeat Datatypes.length
+         HList.polymorphic_list.repeat HList.polymorphic_list.length
+         PrimitivePair.pair._1 PrimitivePair.pair._2] in *;
+    repeat straightline.
+    { eapply (Wf.measure_wf (Z.gt_wf _) Z.of_nat). }
+    { split.
+      { instantiate (1:=O). subst v. rewrite word.unsigned_of_Z. exact eq_refl. }
+      { subst v; rewrite word.add_0_r; split; [ecancel_assumption|]. rewrite word.sub_0_r; auto. } }
+
+    { let e := open_constr:(_) in specialize (H e); destruct H.
+      eapply WeakestPreconditionProperties.Proper_call; repeat intro; cycle 1.
+      { refine (H _ _). }
+      repeat straightline.
+      eexists _, _; repeat straightline.
+      split; repeat straightline.
+      split; repeat straightline.
+      { left; repeat straightline.
+        { subst br'. rewrite unsigned_ltu, Z.ltb_irrefl; trivial. }
+        eexists _, _; repeat straightline.
+        eapply word.if_nonzero, word.eqb_true in H3.
+        instantiate (1:=nil); cbn [Array.array]; split.
+        { ecancel_assumption. }
+        { cbv [getline_io map rev List.app].
+          split; trivial.
+          split.
+          { admit. }
+          split; trivial.
+          eapply f_equal2; f_equal; trivial.
+          change 10 with (byte.unsigned Byte.x0a) in H3.
+          pose proof byte.unsigned_range x2.
+          pose proof byte.unsigned_range Byte.x0a.
+          eapply word.of_Z_inj_small, byte.unsigned_inj in H3; trivial; blia. } }
+
+      (* store *)
+      destruct x as [|x_0 x].
+      { cbn [length] in *.
+        assert (n = x3) as -> by (revert H3; admit).
+        subst br. rewrite unsigned_ltu, Z.ltb_irrefl in H2; case H2; exact eq_refl. }
+      cbn [Array.array] in *.
+      repeat straightline.
+      right; repeat straightline.
+      eexists _, _, _; repeat straightline.
+      { instantiate (1:=x).
+        subst v3.
+        rewrite word.add_assoc.
+        split.
+        { instantiate (1:=S v1). admit. }
+        split; [ecancel_assumption|].
+        cbn [length] in *.
+        (* Require Import ZnWords. ZnWords. *)
+        admit. }
+      { split.
+        { admit. }
+        repeat straightline.
+        (* subroutine return *)
+        subst a.
+        subst v3.
+
+        rename x10 into bs.
+        rename x11 into es.
+        rename x6 into I.
+        rename x3 into _i.
+        rewrite word.add_assoc in H9.
+
+        eexists (byte.of_Z v2::bs), (es).
+        cbn ["$@" "++"].
+        split. { ecancel_assumption. }
+        split; trivial.
+        split.
+        { cbn [length]. rewrite Nat2Z.inj_succ, H11. admit. }
+        split; trivial.
+        subst T a0. cbn. rewrite map_app; cbn.
+        repeat rewrite <-?app_comm_cons, <-?app_assoc; f_equal.
+        f_equal.
+        f_equal.
+        f_equal.
+        subst v2.
+        rewrite word.unsigned_of_Z_nowrap, byte.of_Z_unsigned by admit; trivial. } }
+
+    { (* buffer full *)
+      replace x3 with n in * by admit.
+      exists x, nil; cbn [Array.array].
+      split. { ecancel_assumption. }
+      split. { trivial. }
+      split. { trivial. }
+      assert (length x = O) by admit.
+      split. { admit. }
+      destruct x; cbn [length] in *; try blia; cbn.
+
+      admit. (* <==== TODO: this one is false: if the buffer is full then the I/O trace does not end with newline *)
+    }
+
+    split. { admit. (* leakage *) }
+    subst v.
+    rewrite word.add_0_r in *.
+    split.
+    { ecancel_assumption. }
+    split.
+    { rewrite H5. rewrite word.sub_0_r. trivial. }
+    split.
+    { rewrite H5, H6, word.sub_0_r. admit. }
+    subst t0.
+    trivial.
+
+(* Tue Jul  2 14:26:41 EDT 2024 *)
+Admitted.
+
+Definition maskloop := func! (a) {
+  i = $0;
+  while (i < $2) {
+    mask = $0-((load1(a+i)>>i)&$1);
+    store1(a+i, mask & $123);
+    i = i + $1
+  }
+}.
+
+Require Import coqutil.Map.Interface bedrock2.Map.Separation bedrock2.Map.SeparationLogic.
+
+Instance ctspec_of_maskloop : spec_of "maskloop" :=
+  fun functions => forall k a, exists k_, forall a0 a1 R t m,
+      m =* ptsto a a0 * ptsto (word.add a (word.of_Z 1)) a1 * R ->
+      WeakestPrecondition.call functions "maskloop" k t m [a]
+        (fun k' t' m' rets => rets = [] /\ k' = k_).
+
+Lemma maskloop_ct : program_logic_goal_for_function! maskloop.
+Proof.
+  repeat straightline.
+  eexists nat, lt, (fun i k _ (m : mem) (l : locals) =>
+    map.get l "a" = Some a /\
+    map.get l "i" = Some (word.of_Z (Z.of_nat i)) /\ (
+    i = 0%nat /\ m =* ptsto a a0 * ptsto (word.add a (word.of_Z 1)) a1 * R \/
+    i = 1%nat /\ False \/
+    i = 2%nat /\ False)).
+  Tactics.ssplit; auto using lt_wf.
+  { exists 0%nat; Tactics.ssplit.
+    { subst l0 l; rewrite map.get_put_diff, map.get_put_same; congruence. }
+    { subst l0 l v. rewrite map.get_put_same; trivial. }
+    left; Tactics.ssplit; trivial; ecancel_assumption. }
+  intuition subst.
+Abort.
